\documentclass[12pt]{article}
\usepackage{hyperref}
\usepackage{amsmath}

\begin{document}

\section*{Normalscore v3}

\subsection*{Definition}

\[ t_L \leq h_i \leq t_R \]
\[
s^2 =
\frac{H}{N} \operatorname{Var} (h) + \frac{M}{N} \operatorname{Var} (m) =
\frac{H}{N} \left[
    \langle h^2 \rangle - \langle h \rangle^2
\right] + \Sigma_m
\]

\begin{equation}
\Sigma_m = \int_{(-\infty, t_L) \cup (t_R, \infty)} \left( t - \mu_h \right)^2 n_m(t) \,dt
\label{eq:def_Sigma_m}
\end{equation}

\[
M / N = \int_{(-\infty, t_L) \cup (t_R, \infty)} n_m(t) \,dt
\]

\[
n_m(t) = \frac{1}{\sigma_m\sqrt{2 \pi }} e^{-(t - \mu_h)^2/2\sigma_m^2}, \quad \mu_h = \langle h \rangle
\]

\subsection*{\href{https://en.wikipedia.org/wiki/Normal_distribution}{Normal distribution}}

\[
n(t, \mu, \sigma) = \frac{1}{\sigma\sqrt{2 \pi }} e^{-(t - \mu)^2/2\sigma^2}
\]

\subsection*{\href{https://en.wikipedia.org/wiki/Error_function}{Error function}}

\[
\operatorname{erf} x = \frac{2}{\sqrt{\pi}} \int_{0}^{x} e^{-t^2} \,dt
\quad\quad
\operatorname{erf}'x = \frac{2}{\sqrt{\pi}} e^{-x^{2}}
\]

\subsection*{\href{https://tvims.nsu.ru/chernova/tv/lec/node46.html}{E\(\xi^2\)}}

\[
\text{E}\xi^2 = \frac{1}{\sqrt{2\pi}} \int_{-\infty}^{\infty} x^2 e^{-x^2/2} \,dx =
\frac{2}{\sqrt{2\pi}} \int_{0}^{\infty} x^2 e^{-x^2/2} \,dx =
-\frac{2}{\sqrt{2\pi}} \int_{0}^{\infty} x \,de^{-x^2/2} =
\]

\[
= \left. -\frac{2x}{\sqrt{2\pi}} e^{-x^2/2} \right|_0^\infty +
2 \int_{0}^{\infty} \frac{1}{\sqrt{2\pi}} e^{-x^2/2} \,dx = 0 + 1 = 1
\]

\subsection*{\href{https://en.wikipedia.org/wiki/Variance}{Variance}}

\begin{equation}
\operatorname{Var} (X) = \operatorname {E} \left[(X-\operatorname {E} [X])^{2}\right] = \operatorname {E} \left[X^{2}\right]-\operatorname {E} [X]^{2}
\label{eq:def_Variance}
\end{equation}

\begin{equation}
\operatorname {Var} (X+Y)=\operatorname {Var} (X)+\operatorname {Var} (Y)
\label{eq:def_Variance_sum}
\end{equation}

\pagebreak

\subsection*{Derivation}

Redefine \( M / N \) as follows:
\begin{equation}
M / N = 1 - H / N = 1 - \int_{t_L}^{t_R} n_m(t) \,dt
\end{equation}

Derive \( H / N \):
\[
H / N = \int_{t_L}^{t_R} n_m(t) \,dt =
\int_{t_L}^{t_R} \frac{1}{\sigma_m\sqrt{2\pi}} \exp\left(-\frac{(t - \mu_h)^2}{2\sigma_m^2} \right) \,dt =
\]
\[
= \frac{1}{\sqrt{\pi}} \int_{t_L}^{t_R} \exp\left(-\frac{(t - \mu_h)^2}{2\sigma_m^2} \right) \,d\left(\frac{t - \mu_h}{\sigma_m\sqrt{2}}\right) =
\frac{1}{\sqrt{\pi}} \int_{\tau_L}^{\tau_R} \exp\left(-\tau^2 \right) \,d\tau
\]

Now apply the error function to the above:
\[
\frac{H}{N} = \frac{1}{2}\frac{2}{\sqrt{\pi}} \int_{\tau_L}^{\tau_R} \exp\left(-\tau^2 \right) \,d\tau =
\frac{1}{2} \left( \operatorname{erf} \tau_R - \operatorname{erf} \tau_L \right) , \quad \tau_i = \frac{t_i - \mu_h}{\sigma_m\sqrt{2}}
\]

Using the above, we can derive \(\sigma_m\). If \(t_R = -t_L = t_0\) and \( \mu_h = 0 \) then
\[
H / N = \operatorname{erf}\left(\frac{t_0}{\sigma_m\sqrt{2}}\right)
\]
\[
\operatorname{erf^{-1}}\left(H / N\right) = \frac{t_0}{\sigma_m\sqrt{2}} = \widetilde{\tau}_0
\]
\[
\sigma_m = \frac{t_0}{\operatorname{erf^{-1}}\left(H / N\right)\sqrt{2}} = \frac{t_0}{\widetilde{\tau}_0\sqrt{2}}
\]

Else we can derive \(\sigma_m\) using \href{https://en.wikipedia.org/wiki/Newton%27s_method}{Newton's method}:
\[
f(\sigma_m) = \frac{1}{2} \left[
    \operatorname{erf}\left(\frac{t_R - \mu_h}{\sigma_m\sqrt{2}}\right) -
    \operatorname{erf}\left(\frac{t_L - \mu_h}{\sigma_m\sqrt{2}}\right)
\right] - H / N
\]
\[
f'(\sigma_m) = \frac{1}{\sigma_m^2\sqrt{2\pi}} \left[
    \left(t_L - \mu_h\right) e^{-(t_L - \mu_h)^2/2\sigma_m^2} -
    \left(t_R - \mu_h\right) e^{-(t_R - \mu_h)^2/2\sigma_m^2}
\right]
\]
\[
    x_{n+1}=x_{n}-{\frac {f(x_{n})}{f'(x_{n})}}
\]


Define \( \sigma_m \) using \(\Sigma_m\) \eqref{eq:def_Sigma_m} and \eqref{eq:def_Variance_sum} as follows:
\[
\sigma_m^2 = \int_{-\infty}^{\infty} \left( t - \mu_h \right)^2 n_m(t) \,dt =
\Sigma_m + \int_{t_L}^{t_R} \left( t - \mu_h \right)^2 n_m(t) \,dt
\]

Rearrange:
\[
\Sigma_m = \sigma_m^2 - \int_{t_L}^{t_R} \left( t - \mu_h \right)^2 n_m(t) \,dt
\]
\[
\int_{t_L}^{t_R} \left( t - \mu_h \right)^2 n_m(t) \,dt =
\int_{t_L}^{t_R} \left( t - \mu_h \right)^2 \frac{1}{\sigma_m\sqrt{2 \pi }} \exp\left(-\frac{(t - \mu_h)^2}{2\sigma_m^2} \right) \,dt =
\]
\[
    = \frac{\sigma_m^2}{\sqrt{2\pi}}
    \int_{t_L}^{t_R}
    \left(\frac{t - \mu_h}{\sigma_m}\right)^2
    \exp\left(-\frac{(t - \mu_h)^2}{2\sigma_m^2} \right)
    \,d\left(\frac{t - \mu_h}{\sigma_m}\right) =
\]
\[
    = \frac{\sigma_m^2}{\sqrt{2\pi}}
    \int_{(t_L - \mu_h)/\sigma_m}^{(t_R - \mu_h)/\sigma_m}
    \alpha^2
    \exp\left(-\frac{\alpha^2}{2} \right)
    \,d\alpha = \frac{\sigma_m^2}{\sqrt{2\pi}} I_1
\]

Solve \(I_1\):

\[
    I_1 = 
    \frac{\sqrt{2\pi}}{1}
    \frac{1}{\sqrt{2\pi}}
    \int_{\alpha_L}^{\alpha_R}
    \alpha^2
    \exp\left(-\frac{\alpha^2}{2} \right)
    \,d\alpha =
\]
\[
    = \sqrt{2\pi}
    \left\{
        \left.
        -\frac{x}{\sqrt{2\pi}} e^{-x^2/2}
        \right|_{\alpha_L}^{\alpha_R} +
        \int_{\alpha_L}^{\alpha_R}
        \frac{1}{\sqrt{2\pi}} e^{-x^2/2} \,dx
    \right\} =
\]
\[
    = \sqrt{2\pi}
    \left\{
        -\frac{\alpha_R}{\sqrt{2\pi}} e^{-\alpha_R^2/2} +
        \frac{\alpha_L}{\sqrt{2\pi}} e^{-\alpha_L^2/2} +
        \frac{1}{\sqrt{2\pi}} \int_{\alpha_L}^{\alpha_R}
        e^{-x^2/2} \,dx
    \right\}
\]

Solve the integral:
\[
    \frac{1}{\sqrt{2\pi}} \int_{\alpha_L}^{\alpha_R}
    e^{-x^2/2} \,dx =
    \frac{1}{\sqrt{\pi}} \int_{\alpha_L}^{\alpha_R}
    e^{-x^2/2} \,d\left(\frac{x}{\sqrt{2}}\right) =
\]
\[
    = \frac{1}{\sqrt{\pi}} \int_{\alpha_L/\sqrt{2}}^{\alpha_R/\sqrt{2}}
    e^{-t^2} \,dt =
    \frac{1}{2} \left(
    \operatorname{erf} \tau_R -
    \operatorname{erf} \tau_L
    \right)
\]

\[
    I_1 = \sqrt{2\pi}
    \left[
        -\frac{\tau_R}{\sqrt{\pi}} e^{-\tau_R^2} +
        \frac{\tau_L}{\sqrt{\pi}} e^{-\tau_L^2} +
        \frac{1}{2} \left(
        \operatorname{erf} \tau_R -
        \operatorname{erf} \tau_L
        \right)
    \right]
\]
\[
    = \sqrt{2\pi}
    \left[
        -\frac{\tau_R}{\sqrt{\pi}} e^{-\tau_R^2} +
        \frac{\tau_L}{\sqrt{\pi}} e^{-\tau_L^2} +
        \frac{H}{N}
    \right]
\]

Return back to \(\Sigma_m\):
\[
\Sigma_m = \sigma_m^2 - \frac{\sigma_m^2}{\sqrt{2\pi}} I_1 =
\]
\[
= \sigma_m^2
\left(
    1 +
    \frac{\tau_R}{\sqrt{\pi}} e^{-\tau_R^2} -
    \frac{\tau_L}{\sqrt{\pi}} e^{-\tau_L^2} -
    \frac{H}{N}
\right)
\]

\[
= \sigma_m^2
\left(
    1 + T_R - T_L - H / N
\right)
= \sigma_m^2
\left(
    M / N + \Delta T
\right)
\]

Where

\[
    T_s =
    \frac{1}{\sqrt{\pi}} \frac{t_s}{\sigma_m\sqrt{2}} e^{-\frac{t_s^2}{2\sigma_m^2}} =
    \frac{1}{\sqrt{\pi}} \tau_s e^{-\tau_s^2}
    , \quad
    \Delta T = T_R - T_L
\]

Finally, we have:
\[
s^2 =
H/N \left[
    \langle h^2 \rangle - \langle h \rangle^2
\right] +
\sigma_m^2 (M / N + \Delta T)
\]

\subsection*{Sum of normalscores}

\[
    H = \sum H_i, \quad N = \sum N_i
\]
\[
\frac{H_i}{N} = \frac{H_i(\sigma_m)}{N} = \frac{N_i}{N} \int_{t_{Li}}^{t_{Ri}} n_m(t) \,dt =
\frac{N_i}{2N} \left[ \operatorname{erf}\left(\frac{t_{Ri}}{\sigma_m\sqrt{2}}\right) - \operatorname{erf}\left(\frac{t_{Li}}{\sigma_m\sqrt{2}}\right) \right]
\]

\[
f(\sigma_m) = \sum f_i(\sigma_m), \quad
f'(\sigma_m) = \sum {f_i}'(\sigma_m)
\]

\[
\Sigma_m =
\sigma_m^2
\left\{
    1 + \sum \frac{N_i \Delta T_i}{N} - \sum \frac{H_i}{N}
\right\} =
\frac{\sigma_m^2}{N}
\left\{
    M +
    \sum N_i \Delta T_i
\right\}
\]

\end{document}